mppa_k1c/abstractbb/AbstractBasicBlocksDef.v
@@ -1,5 +1,6 @@
 (** Syntax and Sequential Semantics of Abstract Basic Blocks.
 *)
+Require Import Setoid.
 Require Import ImpPrelude.
 
 Module Type PseudoRegisters.
@@ -303,50 +304,114 @@ Definition list_term_get_hid (l: list_term): hashcode :=
   end.
 
 
-Definition allvalid ge (l: list term) m := forall t, List.In t l -> term_eval ge t m <> None.
+Fixpoint allvalid ge (l: list term) m : Prop :=
+  match l with
+  | nil => True
+  | t::nil => term_eval ge t m <> None
+  | t::l' => term_eval ge t m <> None /\ allvalid ge l' m
+  end. 
 
-Record pseudo_term: Type := {
+Lemma allvalid_extensionality ge (l: list term) m:
+  allvalid ge l m <-> (forall t, List.In t l -> term_eval ge t m <> None).
+Proof.
+  induction l as [|t l]; simpl; try (tauto).
+  destruct l.
+  - intuition (congruence || eauto).
+  - rewrite IHl; clear IHl. intuition (congruence || eauto).
+Qed.
+
+Record pseudo_term: Type := intro_fail {
   mayfail: list term;
   effect: term
 }.
 
-Definition match_pseudo_term (t: term) (pt: pseudo_term) :=
+Definition match_pt (t: term) (pt: pseudo_term) :=
       (forall ge m, term_eval ge t m <> None <-> allvalid ge pt.(mayfail) m)
    /\ (forall ge m0 m1, term_eval ge t m0 = Some m1 -> term_eval ge pt.(effect) m0 = Some m1).
+
+Lemma intro_fail_correct (l: list term) (t: term) :
+   (forall ge m, term_eval ge t m <> None <-> allvalid ge l m) -> match_pt t (intro_fail l t).
+Proof.
+  unfold match_pt; simpl; intros; intuition congruence.
+Qed.
+Hint Resolve intro_fail_correct: wlp.
+
+Definition identity_fail (t: term):= intro_fail [t] t.
+
+Lemma identity_fail_correct (t: term): match_pt t (identity_fail t).
+Proof.
+  eapply intro_fail_correct; simpl; tauto.
+Qed.
+Global Opaque identity_fail.
+Hint Resolve identity_fail_correct: wlp.
+
+Definition nofail (is_constant: op -> bool) (t: term):=
+    match t with
+    | Input x _ => intro_fail ([])%list t
+    | o @ [] => if is_constant o then (intro_fail ([])%list t) else (identity_fail t)
+    | _ => identity_fail t
+    end.
+
+Lemma nofail_correct (is_constant: op -> bool) t:
+ (forall ge o, is_constant o = true -> op_eval ge o nil <> None) -> match_pt t (nofail is_constant t).
+Proof.
+  destruct t; simpl.
+  + intros; eapply intro_fail_correct; simpl; intuition congruence.
+  + intros; destruct l; simpl; auto with wlp.
+    destruct (is_constant o) eqn:Heqo; simpl; intuition eauto with wlp.
+     eapply intro_fail_correct; simpl; intuition eauto with wlp.
+Qed.
+Global Opaque nofail.
+Hint Resolve nofail_correct: wlp.
+
+Definition term_equiv t1 t2:= forall ge m, term_eval ge t1 m = term_eval ge t2 m.
+
+Global Instance term_equiv_Equivalence : Equivalence term_equiv.
+Proof.
+  split; intro x; unfold term_equiv; intros; eauto.
+  eapply eq_trans; eauto.
+Qed.
+
+Lemma match_pt_term_equiv t1 t2 pt: term_equiv t1 t2 -> match_pt t1 pt -> match_pt t2 pt.
+Proof.
+  unfold match_pt, term_equiv.
+  intros H. intuition; try (erewrite <- H1 in * |- *; congruence).
+  erewrite <- H2; eauto; congruence.
+Qed.
+Hint Resolve match_pt_term_equiv: wlp.
+
+Definition app_fail (l: list term) (pt: pseudo_term): pseudo_term :=
+  {| mayfail := List.rev_append l pt.(mayfail); effect := pt.(effect) |}.
+
+Lemma app_fail_correct l pt t1 t2: 
+  match_pt t1 pt -> 
+  match_pt t2 {| mayfail:=t1::l; effect:=t1 |} ->
+  match_pt t2 (app_fail l pt).
+Proof.
+  unfold match_pt in * |- *.
+  intros (XV & XE) (YV & YE).
+  split; intros ge m; try (simpl; auto; fail).
+  generalize (XV ge m) (YV ge m); rewrite !allvalid_extensionality; simpl. clear XV XE YV YE.
+  intuition subst.
+  + rewrite rev_append_rev, in_app_iff, <- in_rev in H3. destruct H3; eauto.
+  + eapply H3; eauto.
+    intros. intuition subst.
+    * eapply H2; eauto. intros; eapply H0; eauto. rewrite rev_append_rev, in_app_iff; auto.
+    * intros; eapply H0; eauto. rewrite rev_append_rev, in_app_iff, <- in_rev; auto.
+Qed.
+Hint Resolve app_fail_correct: wlp.
+Extraction Inline app_fail.
+Global Opaque app_fail.
+
 
 Import ImpCore.Notations.
 Local Open Scope impure_scope.
 
-Record reduction (t:term):= {
-  result:> ?? pseudo_term;
-  result_correct: WHEN result ~> pt THEN match_pseudo_term t pt;
+Record reduction:= {
+  result:> term -> ?? pseudo_term;
+  result_correct: forall t, WHEN result t ~> pt THEN match_pt t pt;
 }.
 Hint Resolve result_correct: wlp.
-
-Program Definition identity_reduce (t: term): reduction t := {| result := RET {| mayfail := [t]; effect := t |} |}.
-Obligation 1.
-  unfold match_pseudo_term, allvalid; wlp_simplify; congruence.
-Qed.
-Global Opaque identity_reduce.
-
-Program Definition failsafe_reduce (is_constant: op -> bool | forall ge o, is_constant o = true -> op_eval ge o nil <> None) (t: term) :=
-  match t with
-  | Input x _ => {| result := RET {| mayfail := []; effect := t |} |}
-  | o @ [] => match is_constant o with 
-              | true => {| result := RET {| mayfail := []; effect := t |} |}
-              | false => identity_reduce t
-              end
-  | _ => identity_reduce t
-  end.
-Obligation 1.
-  unfold match_pseudo_term, allvalid; simpl; wlp_simplify; congruence.
-Qed.
-Obligation 2.
-  unfold match_pseudo_term, allvalid; simpl; wlp_simplify.
-Qed.
-Obligation 3.
-  intuition congruence.
-Qed.
 
 End Terms.
 
